# 지수와 로그 초급 문제 전체 풀이

1. $(\sqrt{16} + \sqrt{25}) \times 2^{(-2)}$
   * $= (4 + 5) \times \frac{1}{4}$
   * $= 9 \times \frac{1}{4} = \frac{9}{4}$

2. $(\sqrt[3]{27} \times \sqrt[3]{64}) \div 3^0$
   * $= (3 \times 4) \div 1$
   * $= 12$

3. $(\sqrt{48} \times \sqrt{75}) \div \sqrt{3}$
   * $= (\sqrt{16 \times 3} \times \sqrt{25 \times 3}) \div \sqrt{3}$
   * $= (4\sqrt{3} \times 5\sqrt{3}) \div \sqrt{3}$
   * $= 20 \times 3 = 60$

4. $(2^3)^{(-1)} \times 4^2 \times \sqrt{9}$
   * $= \frac{1}{8} \times 16 \times 3$
   * $= 6$

5. $\log_2{16} + \log_2{4} \times (\sqrt{16})^0$
   * $= 4 + 2 \times 1$
   * $= 6$

6. $3^2 \times 3^{(-1)} \times \sqrt{9} + \sqrt[3]{8}$
   * $= 9 \times \frac{1}{3} \times 3 + 2$
   * $= 9 + 2 = 11$

7. $(\sqrt{100} + \sqrt{25}) \times 2^{(-1)} - \sqrt[3]{27}$
   * $= (10 + 5) \times \frac{1}{2} - 3$
   * $= \frac{15}{2} - 3 = \frac{9}{2}$

8. $\log_3{27} \times (\sqrt[3]{27})^0 + \log_3{9}$
   * $= 3 \times 1 + 2$
   * $= 5$

9. $(4^2)^{(-1)} \times \sqrt{64} + 2^{(-2)}$
   * $= \frac{1}{16} \times 8 + \frac{1}{4}$
   * $= \frac{1}{2} + \frac{1}{4} = \frac{3}{4}$

10. $(\sqrt{36} + \sqrt[3]{8}) \times 2^0 - \log_2{16}$
    * $= (6 + 2) \times 1 - 4$
    * $= 8 - 4 = 4$

11. $(\log_2{8} + \log_2{2}) \times \sqrt{16} - \log_2{4}$
    * $= (3 + 1) \times 4 - 2$
    * $= 16 - 2 = 8$

12. $(3^2)^{(-1)} \times (\sqrt{9})^2 + \sqrt[3]{125}$
    * $= \frac{1}{9} \times 9 + 5$
    * $= 1 + 5 = 6$

13. $(\sqrt{81} \div \sqrt{9}) \times 3^{(-1)} + \log_2{32}$
    * $= (9 \div 3) \times \frac{1}{3} + 5$
    * $= 1 + 5 = 6$

14. $\log_4{64} + \log_4{4} - (\sqrt[3]{8})^2$
    * $= 3 + 1 - 2^2$
    * $= 4 - 4 = 0$

15. $(2^4)^{(-1)} \times (\sqrt{16})^2 \times 3^0$
    * $= \frac{1}{16} \times 16 \times 1$
    * $= 1$

16. $(\sqrt[3]{125} \times \sqrt[3]{8}) \times 5^{(-1)} + \sqrt{16}$
    * $= (5 \times 2) \times \frac{1}{5} + 4$
    * $= 2 + 4 = 6$

17. $\log_2{32} - \log_2{8} + (\sqrt{9})^0$
    * $= 5 - 3 + 1$
    * $= 3$

18. $(4^{(-2)} \times \sqrt{256}) \div 2^0 + \sqrt[3]{27}$
    * $= (\frac{1}{16} \times 16) \div 1 + 3$
    * $= 1 + 3 = 4$

19. $(\sqrt{144} + \sqrt[3]{27}) \times 3^{(-1)} - \log_3{81}$
    * $= (12 + 3) \times \frac{1}{3} - 4$
    * $= 5 - 4 = 1$

20. $\log_3{81} \times (\sqrt[3]{9})^0 + \log_3{3}$
    * $= 4 \times 1 + 1$
    * $= 5$

21. $(\sqrt{49} + \sqrt{64}) \times 2^{(-2)} \times \sqrt[3]{8}$
    * $= (7 + 8) \times \frac{1}{4} \times 2$
    * $= \frac{15}{4} \times 2 = \frac{15}{2}$

22. $(\sqrt[3]{216} \times \sqrt[3]{27}) \div 3^2 + \sqrt{4}$
    * $= (6 \times 3) \div 9 + 2$
    * $= 2 + 2 = 4$

23. $\log_2{64} + \log_2{8} \times (\sqrt{25})^0$
    * $= 6 + 3 \times 1$
    * $= 9$

24. $4^2 \times 4^{(-1)} \times \sqrt{16} + \sqrt[3]{64}$
    * $= 16 \times \frac{1}{4} \times 4 + 4$
    * $= 16 + 4 = 20$

25. $(\sqrt{225} + \sqrt{36}) \times 2^{(-1)} - \sqrt[3]{125}$
    * $= (15 + 6) \times \frac{1}{2} - 5$
    * $= 10.5 - 5 = 5.5$

26. $\log_4{256} \times (\sqrt[3]{64})^0 + \log_4{16}$
    * $= 4 \times 1 + 2$
    * $= 6$

27. $(5^2)^{(-1)} \times \sqrt{400} + 2^{(-3)}$
    * $= \frac{1}{25} \times 20 + \frac{1}{8}$
    * $= \frac{4}{5} + \frac{1}{8} = \frac{39}{40}$

28. $(\sqrt{121} + \sqrt[3]{216}) \times 2^0 - \log_2{256}$
    * $= (11 + 6) \times 1 - 8$
    * $= 17 - 8 = 9$

29. $(\log_2{16} + \log_2{4}) \times \sqrt{25} - \log_2{8}$
    * $= (4 + 2) \times 5 - 3$
    * $= 30 - 3 = 27$

30. $(4^2)^{(-1)} \times (\sqrt{16})^2 + \sqrt[3]{27}$
    * $= \frac{1}{16} \times 16 + 3$
    * $= 1 + 3 = 4$

31. $(\sqrt{144} \div \sqrt{36}) \times 2^{(-1)} + \log_2{128}$
    * $= (12 \div 6) \times \frac{1}{2} + 7$
    * $= 1 + 7 = 8$

32. $\log_3{243} + \log_3{9} - (\sqrt[3]{27})^2$
    * $= 5 + 2 - 9$
    * $= -2$

33. $(2^5)^{(-1)} \times (\sqrt{32})^2 \times 4^0$
    * $= \frac{1}{32} \times 32 \times 1$
    * $= 1$

34. $(\sqrt[3]{216} \times \sqrt[3]{8}) \times 6^{(-1)} + \sqrt{9}$
    * $= (6 \times 2) \times \frac{1}{6} + 3$
    * $= 2 + 3 = 5$

35. $\log_2{256} - \log_2{32} + (\sqrt{16})^0$
    * $= 8 - 5 + 1$
    * $= 4$

36. $(5^{(-2)} \times \sqrt{225}) \div 3^0 + \sqrt[3]{8}$
    * $= \frac{1}{25} \times 15 \div 1 + 2$
    * $= \frac{3}{5} + 2 = \frac{13}{5}$

37. $(\sqrt{169} + \sqrt[3]{125}) \times 2^{(-1)} - \log_4{256}$
    * $= (13 + 5) \times \frac{1}{2} - 4$
    * $= 9 - 4 = 5$

38. $\log_5{125} \times (\sqrt[3]{25})^0 + \log_5{5}$
    * $= 3 \times 1 + 1$
    * $= 4$

39. $(\sqrt{81} + \sqrt{100}) \times 2^{(-2)} \times \sqrt[3]{27}$
    * $= (9 + 10) \times \frac{1}{4} \times 3$
    * $= \frac{19}{4} \times 3 = \frac{57}{4}$

40. $(\sqrt[3]{343} \times \sqrt[3]{8}) \div 7^2 + \sqrt{16}$
    * $= (7 \times 2) \div 49 + 4$
    * $= \frac{14}{49} + 4 = \frac{210}{49}$

41. $\log_2{128} + \log_2{16} \times (\sqrt{36})^0$
    * $= 7 + 4 \times 1$
    * $= 11$

42. $3^3 \times 3^{(-2)} \times \sqrt{9} + \sqrt[3]{216}$
    * $= 27 \times \frac{1}{9} \times 3 + 6$
    * $= 9 + 6 = 15$

43. $(\sqrt{256} + \sqrt{49}) \times 2^{(-1)} - \sqrt[3]{64}$
    * $= (16 + 7) \times \frac{1}{2} - 4$
    * $= \frac{23}{2} - 4 = \frac{15}{2}$

44. $\log_3{81} \times (\sqrt[3]{125})^0 + \log_3{27}$
    * $= 4 \times 1 + 3$
    * $= 7$

45. $(6^2)^{(-1)} \times \sqrt{324} + 2^{(-2)}$
    * $= \frac{1}{36} \times 18 + \frac{1}{4}$
    * $= \frac{1}{2} + \frac{1}{4} = \frac{3}{4}$

46. $(\sqrt{225} + \sqrt[3]{343}) \times 2^0 - \log_2{128}$
    * $= (15 + 7) \times 1 - 7$
    * $= 22 - 7 = 15$

47. $(\log_2{32} + \log_2{8}) \times \sqrt{9} - \log_2{16}$
    * $= (5 + 3) \times 3 - 4$
    * $= 24 - 4 = 20$

48. $(5^2)^{(-1)} \times (\sqrt{25})^2 + \sqrt[3]{125}$
    * $= \frac{1}{25} \times 25 + 5$
    * $= 1 + 5 = 6$

49. $(\sqrt{196} \div \sqrt{49}) \times 3^{(-1)} + \log_2{64}$
    * $= (14 \div 7) \times \frac{1}{3} + 6$
    * $= \frac{2}{3} + 6 = \frac{20}{3}$

50. $\log_4{256} + \log_4{16} - (\sqrt[3]{64})^2$
    * $= 4 + 2 - 16$
    * $= -10$

51. $(2^6)^{(-1)} \times (\sqrt{64})^2 \times 5^0$
    * $= \frac{1}{64} \times 64 \times 1$
    * $= 1$

52. $(\sqrt[3]{216} \times \sqrt[3]{27}) \times 3^{(-1)} + \sqrt{4}$
    * $= (6 \times 3) \times \frac{1}{3} + 2$
    * $= 6 + 2 = 8$

53. $\log_2{256} - \log_2{64} + (\sqrt{25})^0$
    * $= 8 - 6 + 1$
    * $= 3$

54. $(4^{(-2)} \times \sqrt{144}) \div 2^0 + \sqrt[3]{27}$
    * $= (\frac{1}{16} \times 12) \div 1 + 3$
    * $= \frac{3}{4} + 3 = \frac{15}{4}$

55. $(\sqrt{289} + \sqrt[3]{125}) \times 3^{(-1)} - \log_3{243}$
    * $= (17 + 5) \times \frac{1}{3} - 5$
    * $= \frac{22}{3} - 5 = \frac{7}{3}$

56. $\log_5{125} \times (\sqrt[3]{8})^0 + \log_5{25}$
    * $= 3 \times 1 + 2$
    * $= 5$

57. $(\sqrt{100} + \sqrt{121}) \times 2^{(-2)} \times \sqrt[3]{8}$
    * $= (10 + 11) \times \frac{1}{4} \times 2$
    * $= \frac{21}{4} \times 2 = \frac{21}{2}$

58. $(\sqrt[3]{125} \times \sqrt[3]{216}) \div 5^2 + \sqrt{9}$
    * $= (5 \times 6) \div 25 + 3$
    * $= \frac{30}{25} + 3 = \frac{105}{25}$

59. $\log_2{128} + \log_2{32} \times (\sqrt{16})^0$
    * $= 7 + 5 \times 1$
    * $= 12$

60. $4^2 \times 4^{(-1)} \times \sqrt{25} + \sqrt[3]{216}$
    * $= 16 \times \frac{1}{4} \times 5 + 6$
    * $= 20 + 6 = 26$

61. $(\sqrt{324} + \sqrt{81}) \times 2^{(-1)} - \sqrt[3]{343}$
    * $= (18 + 9) \times \frac{1}{2} - 7$
    * $= \frac{27}{2} - 7 = \frac{13}{2}$

62. $\log_4{256} \times (\sqrt[3]{27})^0 + \log_4{64}$
    * $= 4 \times 1 + 3$
    * $= 7$

63. $(7^2)^{(-1)} \times \sqrt{441} + 2^{(-3)}$
    * $= \frac{1}{49} \times 21 + \frac{1}{8}$
    * $= \frac{21}{49} + \frac{1}{8} = \frac{217}{392}$

64. $(\sqrt{144} + \sqrt[3]{125}) \times 2^0 - \log_2{256}$
    * $= (12 + 5) \times 1 - 8$
    * $= 17 - 8 = 9$

65. $(\log_2{64} + \log_2{16}) \times \sqrt{9} - \log_2{32}$
    * $= (6 + 4) \times 3 - 5$
    * $= 30 - 5 = 25$

66. $(3^3)^{(-1)} \times (\sqrt{27})^2 + \sqrt[3]{64}$
    * $= \frac{1}{27} \times 27 + 4$
    * $= 1 + 4 = 5$

67. $(\sqrt{225} \div \sqrt{25}) \times 2^{(-1)} + \log_2{128}$
    * $= (15 \div 5) \times \frac{1}{2} + 7$
    * $= \frac{3}{2} + 7 = \frac{17}{2}$

68. $\log_3{243} + \log_3{27} - (\sqrt[3]{125})^2$
    * $= 5 + 3 - 25$
    * $= -17$

69. $(2^5)^{(-1)} \times (\sqrt{128})^2 \times 3^0$
    * $= \frac{1}{32} \times 128 \times 1$
    * $= 4$

70. $(\sqrt[3]{216} \times \sqrt[3]{125}) \times 6^{(-1)} + \sqrt{16}$
    * $= (6 \times 5) \times \frac{1}{6} + 4$
    * $= 5 + 4 = 9$

71. $\log_2{256} - \log_2{64} + (\sqrt{36})^0$
    * $= 8 - 6 + 1$
    * $= 3$

72. $(5^{(-2)} \times \sqrt{400}) \div 2^0 + \sqrt[3]{27}$
    * $= (\frac{1}{25} \times 20) \div 1 + 3$
    * $= \frac{4}{5} + 3 = \frac{19}{5}$

73. $(\sqrt{196} + \sqrt[3]{216}) \times 3^{(-1)} - \log_4{256}$
    * $= (14 + 6) \times \frac{1}{3} - 4$
    * $= \frac{20}{3} - 4 = \frac{8}{3}$

74. $\log_5{125} \times (\sqrt[3]{64})^0 + \log_5{25}$
    * $= 3 \times 1 + 2$
    * $= 5$

75. $(\sqrt{144} + \sqrt{169}) \times 2^{(-2)} \times \sqrt[3]{8}$
    * $= (12 + 13) \times \frac{1}{4} \times 2$
    * $= \frac{25}{4} \times 2 = \frac{25}{2}$

76. $(\sqrt[3]{343} \times \sqrt[3]{27}) \div 7^2 + \sqrt{25}$
    * $= (7 \times 3) \div 49 + 5$
    * $= \frac{21}{49} + 5 = \frac{266}{49}$

77. $\log_2{256} + \log_2{64} \times (\sqrt{9})^0$
    * $= 8 + 6 \times 1$
    * $= 14$

78. $5^2 \times 5^{(-1)} \times \sqrt{16} + \sqrt[3]{125}$
    * $= 25 \times \frac{1}{5} \times 4 + 5$
    * $= 20 + 5 = 25$

79. $(\sqrt{289} + \sqrt{100}) \times 2^{(-1)} - \sqrt[3]{216}$
    * $= (17 + 10) \times \frac{1}{2} - 6$
    * $= \frac{27}{2} - 6 = \frac{15}{2}$

80. $\log_4{256} \times (\sqrt[3]{216})^0 + \log_4{32}$
    * $= 4 \times 1 + \frac{5}{2}$
    * $= \frac{13}{2}$

81. $(6^2)^{(-1)} \times \sqrt{324} + 2^{(-2)}$
    * $= \frac{1}{36} \times 18 + \frac{1}{4}$
    * $= \frac{1}{2} + \frac{1}{4} = \frac{3}{4}$

82. $(\sqrt{256} + \sqrt[3]{125}) \times 3^0 - \log_2{128}$
    * $= (16 + 5) \times 1 - 7$
    * $= 21 - 7 = 14$

83. $(\log_2{128} + \log_2{32}) \times \sqrt{4} - \log_2{64}$
    * $= (7 + 5) \times 2 - 6$
    * $= 24 - 6 = 18$

84. $(4^2)^{(-1)} \times (\sqrt{36})^2 + \sqrt[3]{27}$
    * $= \frac{1}{16} \times 36 + 3$
    * $= \frac{9}{4} + 3 = \frac{21}{4}$

85. $(\sqrt{196} \div \sqrt{49}) \times 2^{(-1)} + \log_2{256}$
    * $= (14 \div 7) \times \frac{1}{2} + 8$
    * $= 1 + 8 = 9$

86. $\log_3{243} + \log_3{81} - (\sqrt[3]{64})^2$
    * $= 5 + 4 - 16$
    * $= -7$

87. $(2^6)^{(-1)} \times (\sqrt{256})^2 \times 2^0$
    * $= \frac{1}{64} \times 256 \times 1$
    * $= 4$

88. $(\sqrt[3]{125} \times \sqrt[3]{216}) \times 5^{(-1)} + \sqrt{9}$
    * $= (5 \times 6) \times \frac{1}{5} + 3$
    * $= 6 + 3 = 9$

89. $\log_2{256} - \log_2{32} + (\sqrt{25})^0$
    * $= 8 - 5 + 1$
    * $= 4$

90. $(4^{(-2)} \times \sqrt{324}) \div 3^0 + \sqrt[3]{8}$
    * $= (\frac{1}{16} \times 18) \div 1 + 2$
    * $= \frac{9}{8} + 2 = \frac{25}{8}$

91. $(\sqrt{225} + \sqrt[3]{343}) \times 2^{(-1)} - \log_3{81}$
    * $= (15 + 7) \times \frac{1}{2} - 4$
    * $= 11 - 4 = 7$

92. $\log_5{125} \times (\sqrt[3]{27})^0 + \log_5{125}$
    * $= 3 \times 1 + 3$
    * $= 6$

93. $(\sqrt{144} + \sqrt{100}) \times 2^{(-2)} \times \sqrt[3]{27}$
    * $= (12 + 10) \times \frac{1}{4} \times 3$
    * $= \frac{22}{4} \times 3 = \frac{66}{4}$

94. $(\sqrt[3]{216} \times \sqrt[3]{125}) \div 6^2 + \sqrt{16}$
    * $= (6 \times 5) \div 36 + 4$
    * $= \frac{30}{36} + 4 = \frac{174}{36}$

95. $\log_2{128} + \log_2{16} \times (\sqrt{49})^0$
    * $= 7 + 4 \times 1$
    * $= 11$

96. $3^3 \times 3^{(-2)} \times \sqrt{25} + \sqrt[3]{64}$
    * $= 27 \times \frac{1}{9} \times 5 + 4$
    * $= 15 + 4 = 19$

97. $(\sqrt{324} + \sqrt{81}) \times 2^{(-1)} - \sqrt[3]{216}$
    * $= (18 + 9) \times \frac{1}{2} - 6$
    * $= \frac{27}{2} - 6 = \frac{15}{2}$

98. $\log_4{256} \times (\sqrt[3]{125})^0 + \log_4{16}$
    * $= 4 \times 1 + 2$
    * $= 6$

99. $(5^2)^{(-1)} \times \sqrt{400} + 2^{(-3)}$
    * $= \frac{1}{25} \times 20 + \frac{1}{8}$
    * $= \frac{4}{5} + \frac{1}{8} = \frac{39}{40}$

100. $(\sqrt{196} + \sqrt[3]{343}) \times 2^0 - \log_2{256}$
     * $= (14 + 7) \times 1 - 8$
     * $= 21 - 8 = 13$


<script type="text/javascript" src="http://cdn.mathjax.org/mathjax/latest/MathJax.js?config=TeX-AMS-MML_HTMLorMML"></script>
<script type="text/x-mathjax-config">
  MathJax.Hub.Config({
    tex2jax: {inlineMath: [['$', '$']]},
    messageStyle: "none",
    "HTML-CSS": { availableFonts: "TeX", preferredFont: "TeX" },
  });
</script>